formalization/MailboxActors/MailboxActors/Examples/Anoma/Ordering/Executor/Behaviour.lean
@@ -45,23 +45,20 @@ def executorReadReplyAction
     localState := { st with
       completedReads := st.completedReads ++ [w.1] } }
 
-def executorActions
-    : @Behaviour (S A) AnomaIdx.executor :=
+def executorActions : @Behaviour (S A) AnomaIdx.executor :=
   letI := S A
   [ { Witness := A.KVSKey × A.KVSDatum
       guard := executorReadReplyGuard A
       action := executorReadReplyAction A } ]
 
-private
-theorem executorNonOverlapping
-    : @NonOverlappingGuards (S A) _ (executorActions A) := by
+private theorem executorNonOverlapping :
+    @NonOverlappingGuards (S A) _ (executorActions A) := by
   letI := S A
   intro inp
   simp only [executorActions, List.filter]
   split <;> simp
 
-def executorBehaviour
-    : @WellFormedBehaviour (S A) AnomaIdx.executor :=
+def executorBehaviour : @WellFormedBehaviour (S A) AnomaIdx.executor :=
   letI := S A
   { actions := executorActions A
     nonOverlapping := executorNonOverlapping A }
